Hoare/Hoare_Semi_Indexed_Sound2.thy
@@ -1,0 +1,372 @@
+theory Hoare_Indexed_Sound2 imports Hoare_Indexed Hoare
+begin
+
+(*
+ * Here we show that the Hoare logic with explicit step-indexes defined in
+ * Hoare_Indexed.thy is sound with respect to the one defined in Hoare.thy.
+ * I do not believe the indexed Hoare logic is complete with respect to the non-indexed one,
+ * but this doesn't really matter since its use is primarily in making it easier to prove
+ * certain Hoare rules which are to be used in a non-indexed setting.
+ *)
+
+(* Wrapping the indexed Hoare triples to make them work like non-indexed ones.
+ * The idea here is that we only care about how long the "output" (program combined with
+ * the arbitrary tail quantified within the Hoare triple definition) is safe for. So, in order
+ * for this to work like a normal Hoare triple, for any desired safe execution length npre,
+ * we must be able to find a suffix execution
+ * (safe for some npost number of steps) such that the concatenation is safe for npre. *)
+definition HT' :: "('syn, 'mstate) semc \<Rightarrow> ('mstate \<Rightarrow> bool) \<Rightarrow> 'syn gensyn list \<Rightarrow> ('mstate \<Rightarrow> bool)\<Rightarrow> bool" where
+"HT' gs P c Q =
+  ((\<forall> n . |#gs#| {#- P, (n) -#} c {#- Q, n -#}))"
+
+lemma HT'I :
+  assumes H : "(\<And> n. |#gs#| {#- P, (n) -#} c {#- Q, n -#})"
+  shows "HT' gs P c Q" using assms unfolding HT'_def by blast
+
+lemma HT'D :
+  assumes H : "HT' gs P c Q"
+  shows "|#gs#| {#- P, n -#} c {#- Q, n -#}"
+  using H unfolding HT'_def by simp
+
+lemma safe_imp_safe_for :
+  assumes H: "safe gs m"
+  shows "safe_for gs m n" using H
+proof(induction n arbitrary: m)
+  case 0
+
+  have Ex0 : "sem_exec_p gs m m"
+    unfolding sem_exec_p_def by auto
+
+  have Nostep : "sem_exec_c_p gs m 0 m" 
+      by(auto intro: sem_exec_c_p.intros)
+
+  have "imm_safe gs m" using safeD[OF 0 Ex0]
+    by simp
+
+  then consider (1) "cont m = Inl []"  |
+                (2) m' where "(sem_step_p gs m m')"
+    unfolding imm_safe_def by blast
+  then show ?case
+  proof cases
+    case 1
+
+    have "sem_exec_c_p gs m 0 m" 
+      by(auto intro: sem_exec_c_p.intros)
+
+    then show ?thesis using 1 unfolding safe_for_def by blast
+  next
+    case 2
+
+    then obtain h t where Cons : "cont m = Inl (h#t)"
+      unfolding sem_step_p_eq
+      by(auto simp add: sem_step_def split: list.splits sum.splits)
+
+    show ?thesis using Cons Nostep unfolding safe_for_def by blast
+  qed
+next
+  case (Suc n)
+
+  have Ex0 : "sem_exec_p gs m m"
+    unfolding sem_exec_p_def by auto
+
+  have "imm_safe gs m" using safeD[OF Suc.prems Ex0]
+    by simp
+
+  then consider (A) "cont m = Inl []"  |
+                (B) m' where "(sem_step_p gs m m')"
+    unfolding imm_safe_def by blast
+  then show ?case
+  proof cases
+    case A
+
+    have "sem_exec_c_p gs m 0 m" 
+      by(auto intro: sem_exec_c_p.intros)
+
+    then show ?thesis using A unfolding safe_for_def by blast
+  next
+    case B
+
+    then have Exec : "sem_exec_p gs m m'"
+      unfolding sem_exec_p_def by auto
+
+    have Safe: "safe gs m'" using safe_exec_safe[OF Suc.prems Exec] by simp
+
+    have "safe_for gs m' n" using Suc.IH[OF Safe] by simp
+
+    then consider (B1) n0 full' where "n0 \<le> n" "sem_exec_c_p gs m' n0 full'" "cont full' = Inl []" |
+                  (B2) "\<And> n0 . n0\<le>n \<Longrightarrow> \<exists>full' h t. sem_exec_c_p gs m' n0 full' \<and> cont full' = Inl (h # t)"
+      unfolding safe_for_def
+      by blast
+
+    then show ?thesis 
+    proof cases
+      case B1
+
+      have Conc1 : "(Suc n0) \<le> Suc n" using B1 by simp
+
+      have Conc2 : "sem_exec_c_p gs m (Suc n0) full'" 
+        using Excp_Suc[OF B B1(2)] by simp
+
+      show ?thesis unfolding safe_for_def
+        using Conc1 Conc2 B1(3)
+        by blast
+    next
+      case B2
+
+      have Conc' : "\<And> n0 . n0\<le>Suc n \<Longrightarrow> \<exists>full' h t. sem_exec_c_p gs m n0 full' \<and> cont full' = Inl (h # t)"
+      proof-
+        fix n0
+        assume N0 : "n0 \<le> Suc n"
+        show "\<exists>full' h t. sem_exec_c_p gs m n0 full' \<and> cont full' = Inl (h # t)"
+        proof(cases n0)
+          case Z' : 0
+
+          have Conc1 : "sem_exec_c_p gs m 0 m" 
+            by(auto intro: sem_exec_c_p.intros)
+
+          obtain h t where Conc2 : "cont m = Inl (h#t)"
+            using B
+            unfolding sem_step_p_eq
+            by(auto simp add: sem_step_def split: list.splits sum.splits)
+
+          show ?thesis using Conc1 Conc2 unfolding Z' by blast
+        next
+          case Suc' : (Suc n0')
+
+          have N0'_n : "n0' \<le> n" using N0 Suc'
+            by auto
+
+          obtain full' h t where Tail_exec : "sem_exec_c_p gs m' n0' full'" 
+            and Tail_cont : "cont full' = Inl (h # t)"
+            using B2[OF N0'_n] by blast
+
+          have Full_Exec : "sem_exec_c_p gs m (Suc n0') full'"
+            using Excp_Suc[OF B Tail_exec] by simp
+
+          then show ?thesis using Tail_cont unfolding Suc' by blast
+        qed
+      qed
+
+      then show ?thesis
+        unfolding safe_for_def
+        by blast
+    qed
+  qed
+qed
+
+lemma safe_for_imm_safe :
+  assumes H : "safe_for gs m n"
+  assumes H' : "sem_exec_c_p gs m n m'"
+  shows "imm_safe gs m'"
+proof-
+
+  consider 
+    (1) n0 m'_alt where "n0 \<le> n" "sem_exec_c_p gs m n0 m'_alt" "cont m'_alt = Inl []" |
+    (2) "\<And> n0 . n0 \<le>n  \<Longrightarrow> \<exists>m'_alt h t. sem_exec_c_p gs m n0 m'_alt \<and> cont m'_alt = Inl (h # t)"
+    using H unfolding safe_for_def
+    by blast
+
+  then show "imm_safe gs m'"
+  proof cases
+    case 1
+
+    obtain m2 where Exec_start : "sem_exec_c_p gs m n0 m2"
+              and Exec_finish : "sem_exec_c_p gs m2 (n - n0) m'"
+      using exec_c_p_split[OF H' 1(1)]
+      by blast
+
+    have M2_m'_alt : "m2 = m'_alt"
+      using exec_c_p_determ[OF 1(2) Exec_start] by simp
+
+    (* idea: if n0 = n, we are done *)
+    show ?thesis
+    proof(cases "n0 = n")
+      case True
+
+      have Exec_alt_n : "sem_exec_c_p gs m n m'_alt"
+        using 1 unfolding True by simp
+
+      have M'_eq : "m'_alt = m'"
+        using exec_c_p_determ[OF H' Exec_alt_n] by auto
+
+      then show ?thesis using 1 unfolding imm_safe_def M'_eq by blast
+    next
+      (* otherwise we have a contradiction, since we need to execute past an Inl [] *)
+      case False
+
+      have Leq' : "1 \<le> n - n0"
+        using False 1(1) by auto
+
+      obtain mbad where Bad: "sem_exec_c_p gs m2 1 mbad"
+        using exec_c_p_split[OF Exec_finish Leq'] by blast
+
+      have Bad_step : "sem_step_p gs m2 mbad"
+        using Excp_1'[OF Bad] by simp
+
+      then obtain bad_h bad_t where Bad_nonnil : "cont m2 = Inl (bad_h#bad_t)"
+        unfolding sem_step_p_eq
+        by(auto simp add: sem_step_def split: sum.splits list.splits)
+
+      hence False using 1(3) unfolding M2_m'_alt by simp
+
+      then show ?thesis by simp
+    qed
+  next
+    case 2
+
+    obtain m'_alt h t where Exec_alt : "sem_exec_c_p gs m n m'_alt" and Cont_alt : "cont m'_alt = Inl (h # t)"
+      using 2[of n] by blast
+
+    have Eq : "m'_alt = m'" using exec_c_p_determ[OF H' Exec_alt] by simp
+
+    obtain m'a where "sem_step_p gs m' m'a"
+      using Cont_alt Exec_alt
+      unfolding imm_safe_def Eq sem_step_p_eq sem_step_def
+      by(cases h; auto)
+
+    then show ?thesis unfolding imm_safe_def by blast
+  qed
+qed
+
+
+lemma HT'_imp_HT :
+  assumes H : "HT' gs P c Q"
+  shows "|gs| {-P-} c {-Q-}"
+proof
+  fix c'
+  assume Guard : "|gs| {Q} c'"
+  show "|gs| {P} (c @ c')"
+  proof
+    fix m :: "('a, 'b) control"
+    assume Pm : "P (payload m)" 
+    assume Cm : "cont m = Inl (c @ c')" 
+    show "safe gs m"
+    proof
+      fix m'
+      assume Exec : "sem_exec_p gs m m'" 
+
+      obtain n where Execc : "sem_exec_c_p gs m n m'"
+        using exec_p_imp_exec_c_p[OF Exec] by auto
+
+      obtain npost where Npost : "|#gs#| {#-P, n-#} c {#-Q, npost-#}" using HT'D[OF H, of n]
+        by blast
+
+      have Guard'_out : "|#gs#| {#Q, npost#} c'"
+      proof
+        fix mx :: "('a, 'b) control"
+        assume Q: "Q (payload mx)"
+        assume C: "cont mx = Inl c'" 
+
+        have Safe : "safe gs mx"
+          using guardedD[OF Guard Q C] by simp
+
+        show "safe_for gs mx npost"
+          using safe_imp_safe_for[OF Safe] by simp
+      qed
+
+      have Guard'_in : "|#gs#| {#P, n#} (c @ c')"
+        using HTiE[OF Npost Guard'_out] by simp
+
+      have Safe' : "safe_for gs m n"
+        using guardediD[OF Guard'_in Pm Cm] by simp
+
+      show "imm_safe gs m'"
+        using safe_for_imm_safe[OF Safe' Execc] by simp
+    qed
+  qed
+qed
+
+(* Work in progress - concept for a limited completeness theorem, sufficient for HWhile *)
+
+lemma HT_imp_HT' :
+  assumes H : "|gs| {-P-} c {-Q-}"
+  shows "HT' gs P c Q"
+  unfolding HT'_def
+proof
+  fix n
+
+  show "|#gs#| {#-P, n-#} c {#-Q, n-#}"
+  proof
+    fix c'
+    assume "|#gs#| {#Q, n#} c'"
+    show "|#gs#| {#P, n#} (c @ c')"
+    proof
+      fix m :: "('a, 'b) control"
+
+      assume "P (payload m)"
+      assume "cont m = Inl (c @ c') "
+      show "safe_for gs m n"
+        using HTE[OF H]
+
+  proof(induction n arbitrary: c)
+    case 0
+    then show ?case sorry
+  next
+    case (Suc n)
+    show ?case
+    proof(rule HTiI)
+      fix c'
+      assume X:  "|#gs#| {#Q, Suc n#} c'"
+      hence X' : "|#gs#| {#Q, n#} c'" sorry
+
+      have Conc' :  "|#gs#| {#P, n#} (c @ c')"
+        using HTiE[OF Suc.IH[OF Suc.prems] X']
+        by auto
+
+
+
+      show "|#gs#| {#P, Suc n#} (c @ c')" using HTE[OF Suc.prems]
+(* if c' unsafe under Q, then we can find a smallest n where it is not safe for n steps
+ * 
+ *)
+  qed
+
+  show "\<exists> npost . |#gs#| {#-P, npre-#} c {#-Q, npost-#}"  using HTE[OF H]
+  
+
+  show "\<exists> npost . |#gs#| {#-P, npre-#} c {#-Q, npost-#}"  using H
+  proof(induction npre arbitrary: c)
+    case 0
+    then show ?case  sorry (* a = 0 should work here. *)
+  next
+    case (Suc npre)
+
+    obtain ahyp where Ahyp : "|#gs#| {#-P, npre-#} c {#-Q, ahyp-#}"
+      using Suc.IH[OF Suc.prems]
+      by blast
+
+    show ?case using HTiE[OF Ahyp]
+  qed
+
+  have Conc' : "\<And> npost . |#gs#| {#-P, npre-#} c {#-Q, npost-#}"
+  proof
+    fix npost c'
+    assume Gdi : "|#gs#| {#Q, npost#} c'"
+
+(* idea: what does it mean that we fail starting at Q?
+ *)
+
+    have Meh : "|gs| {Q} c'"
+    proof
+      fix m :: "('a, 'b) control"
+      assume Q : "Q (payload m)"
+      assume Cntn : "cont m = Inl c'"
+      show "safe gs m" using Gdi Q Cntn
+      proof(induction 
+
+
+
+    show "|#gs#| {#P, npre#} (c @ c')"
+      using guardediD[OF Gdi] HTE[OF H]
+
+
+(* idea: if no valid npost exists, then it must be the case that for this npre,
+ * there is no way to get the whole program to be safe for that many steps.
+ *)
+
+  show "\<exists> npost . |#gs#| {#-P, npre-#} c {#-Q, npost-#}" 
+  proof
+qed
+
+
+end
