Hoare/Hoare_Step.thy
@@ -58,7 +58,228 @@ definition no_control_l :: "
    * for all _other_ semantics. no_control_lifting should do the rest. i think.
  *)
 
+(* can we get away with lift_pred_s? looks like the answer is no; see below. *)
+
+(* YOU ARE HERE.
+   The main thing i am trying to figure out now is how big of an issue this is.
+   on the one hand it means that these rules might not naturally compose between
+   different liftings (which will have different valid sets).
+
+   A weaker, alternate notion of lifting validity (updates are only guaranteed to be in
+   the valid set if we started in the valid set) feels very ugly, but i worry i am running
+   out of other options.
+*)
+
 lemma HTS_imp_HT' :
+  assumes H: "f % {{P1}} c {{P2}}"
+  assumes Valid : "lifting_validx l S"
+  assumes Hf' : "f' = no_control_l l f"
+  assumes H0 : "gs = pcomps fs"
+  assumes Hpres : "sups_pres (set fs)"
+  assumes Hseq : "seq_sem_l_gen lfts \<in> set fs"
+  assumes Skip : "lfts c = Sskip"
+  assumes Hnemp : "g \<in> (set fs - {seq_sem_l_gen lfts})"
+  assumes Hdom : "(f' \<downharpoonleft> (set fs - {seq_sem_l_gen lfts}) c)"
+  shows "|gs| {~ (lift_pred_validx_s id l S c P1) ~} [G c z] {~ (lift_pred_validx_s id l S c P2) ~}"
+proof(rule HT'I)
+  fix npost
+
+  have Valid' : "lifting_valid l S"
+    using lifting_validxDV[OF Valid] by auto
+
+  have "|#gs#| {#-lift_pred_validx_s id l S c
+                     P1, (0 +
+                          npost)-#} [G c z] {#-lift_pred_validx_s id l S c
+       P2, npost-#}"
+    unfolding add_0
+  proof
+    fix c'
+
+    assume Guard : "|#gs#| {#lift_pred_validx_s id l S c P2, npost#} c'"
+    show "|#gs#| {#lift_pred_validx_s id l S c P1, npost#} ([G c z] @ c')"
+    proof
+      fix m :: "('a, 'c) control"
+      assume Hpay : "lift_pred_validx_s id l S c P1 (payload m)"
+      assume Hcont : "cont m = Inl ([G c z] @ c') "
+
+      have Hpay1 : "P1 (LOut l c (payload m))" and Hpay2 : "payload m \<in> S c" and Hpay3 : "payload m \<in> ok_S"
+        using Hpay lifting_validxDS[OF Valid]
+        unfolding lift_pred_valid_s_def lift_pred_validx_s_def lift_pred_s_def
+        by auto
+
+      have Hpay' : "P2 (f c (LOut l c (payload m)))"
+        using HTSE[OF H Hpay1]
+        by simp
+
+      show "safe_for gs m npost"
+      proof(cases "(sem_step gs m)")
+        case (Inr bad)
+  
+        then have False using Hcont H0
+          by(auto simp add: sem_step_def)
+  
+        then show ?thesis by auto
+      next
+        case (Inl m')
+
+        have Pres' : "sups_pres (set fs - {seq_sem_l_gen lfts})"
+          using sups_pres_subset[OF Hpres, of "set fs - {seq_sem_l_gen lfts}"] by auto
+
+        obtain fs_sub where Fs_sub : "set fs_sub = set fs - {seq_sem_l_gen lfts}"
+          using finite_list[of "set fs - {seq_sem_l_gen lfts}"]
+          by auto
+
+(* ok, so the idea now is:
+- we know full step (op + control flow) leads to m'
+- dominance over everything but the seq means we can treat it as
+  "op (dominant thing) then seq"
+- we can then unfold these things in order and everything should be ok.
+*)
+
+        have Assoc : 
+             "pcomps (fs_sub @ [seq_sem_l_gen lfts]) =
+              pcomps [pcomps fs_sub, pcomps [seq_sem_l_gen lfts]]"
+        proof(rule pcomps_assoc)
+
+          have "set fs - {seq_sem_l_gen lfts} \<union> set [seq_sem_l_gen lfts] = set fs"
+            using Hseq 
+            by(simp; blast)
+
+          then show "sups_pres (set fs_sub \<union> set [seq_sem_l_gen lfts])"
+            unfolding Fs_sub
+            using Hpres
+            by auto
+        next
+
+          have "set fs_sub \<noteq> {}" using Hnemp unfolding Fs_sub by auto
+
+          then show "fs_sub \<noteq> []" by auto
+        next
+
+          show "[seq_sem_l_gen lfts] \<noteq> []" by simp
+        qed
+
+        have Set_alt : "set (fs_sub @ [seq_sem_l_gen lfts]) = set fs"
+          unfolding set_append Fs_sub
+          using Un_Diff_cancel2 Hseq
+          by auto
+
+        have Gs_alt : "gs = pcomps (fs_sub @ [seq_sem_l_gen lfts])"
+          using pcomps_set_eq[OF Hpres Hseq _ Set_alt, of fs] H0
+          by auto
+          
+(* TODO: find a better solution than this awful type annotation hack *)
+        have Seq_pres : 
+          "sups_pres {(seq_sem_l_gen lfts  :: ('a \<Rightarrow> 'a gensyn list md_triv option md_prio \<times>
+            String.literal md_triv option md_prio \<times> 'c
+            \<Rightarrow> 'a gensyn list md_triv option md_prio \<times>
+               String.literal md_triv option md_prio \<times>
+               'c))}"
+          using sups_pres_subset[OF Hpres, of "{seq_sem_l_gen lfts}"] Hseq
+          by(auto)
+
+
+        have Gs_alt' : "gs = pcomps [pcomps fs_sub, seq_sem_l_gen lfts]"
+          using Gs_alt pcomps_singleton[OF Seq_pres, of "[seq_sem_l_gen lfts]"]
+          unfolding Assoc
+          unfolding append.simps H0
+          by auto
+
+        have Hdom' :  "f' \<downharpoonleft> (set fs_sub) c"
+          using Fs_sub Hdom by auto
+        have Dominate1 : "pcomps fs_sub c m = f' c m" using dominant_pcomps[OF _ _ Hdom', of g m] Pres' Hnemp Fs_sub
+          by auto
+
+(* almost have this. the missing ingredient is using the fact that
+ * information content will increase (for a strong-valid lifting) *)
+
+(* TODO: declare a lemmas with all the definitions of liftings... *)
+        obtain pri1 pri2 rest where Msplit :
+          "m = (mdp pri1 (Some (mdt (G c z # c'))), mdp pri2 None, rest)"
+          and Rest : "rest \<in> ok_S"
+          using Gs_alt' Dominate1 Skip Hpay Hcont Hf'
+          by(auto simp add: seq_sem_l_gen_def seq_sem_lifting_gen_def 
+            lift_pred_valid_s_def lift_pred_validx_s_def lift_pred_s_def
+            no_control_lifting_def cont_def
+            schem_lift_defs fst_l_def snd_l_def prio_l_def triv_l_def option_l_def seq_sem_def
+            prod_bsup no_control_l_def
+            split: md_prio.splits prod.splits md_triv.splits option.splits list.split_asm)
+
+        have Rest' : "rest \<in> S c"
+          using lifting_validxDS[OF Valid] Rest by auto
+
+        have LUpd_rest1 :
+          "rest <[ LUpd l c (f c (LOut l c rest)) rest"
+          using lifting_validDI[OF Valid' Rest']
+          by auto
+
+        have LUpd_rest2 : "[^ LUpd l c (f c (LOut l c rest)) rest, rest ^] = LUpd l c (f c (LOut l c rest)) rest"
+          using bsup_base_leq2[OF LUpd_rest1]
+          by simp
+
+        then have LOut_m : "LOut (no_control_lifting l) c (gs c m) = LOut (no_control_lifting l) c (f' c m)"
+          using Gs_alt' Dominate1 Skip Hpay Hcont Hf' Msplit
+          by(auto simp add: seq_sem_l_gen_def seq_sem_lifting_gen_def 
+            lift_pred_valid_s_def lift_pred_s_def
+            no_control_lifting_def cont_def
+            schem_lift_defs fst_l_def snd_l_def prio_l_def triv_l_def option_l_def seq_sem_def
+            prod_bsup no_control_l_def
+            split: md_prio.splits prod.splits md_triv.splits option.splits list.split_asm)
+
+
+(* key sub-result. *)
+        have Pay_final : "payload m' = LUpd l c (f c (LOut l c (payload m))) (payload m)"
+          using Gs_alt' Dominate1 Skip Hpay Hcont Hf' Msplit Inl LUpd_rest2
+          by(auto simp add: seq_sem_l_gen_def seq_sem_lifting_gen_def sem_step_def
+            lift_pred_valid_s_def lift_pred_s_def
+            no_control_lifting_def cont_def
+            schem_lift_defs fst_l_def snd_l_def prio_l_def triv_l_def option_l_def seq_sem_def
+            prod_bsup no_control_l_def
+            split: md_prio.splits prod.splits md_triv.splits option.splits list.split_asm)
+
+(* key sub-result. idea here is that no_control_l means we won't overwrite. *)
+        have Cont_final : "cont m' = cont (seq_sem_l_gen lfts c m)"
+          using Hcont Msplit Skip Inl Gs_alt' Dominate1 Hf'
+          by(auto simp add: seq_sem_l_gen_def seq_sem_lifting_gen_def sem_step_def
+            lift_pred_valid_s_def lift_pred_s_def
+            no_control_lifting_def cont_def
+            schem_lift_defs fst_l_def snd_l_def prio_l_def triv_l_def option_l_def seq_sem_def
+            prod_bsup no_control_l_def prio_bsup option_bsup leq_refl
+            split: md_prio.splits prod.splits md_triv.splits option.splits list.split_asm)         
+
+        hence Cont_final' : "cont m' = Inl c'"
+          using Hcont Msplit Skip
+          by(auto simp add: seq_sem_l_gen_def seq_sem_lifting_gen_def sem_step_def
+            lift_pred_valid_s_def lift_pred_s_def
+            no_control_lifting_def cont_def
+            schem_lift_defs fst_l_def snd_l_def prio_l_def triv_l_def option_l_def seq_sem_def
+            prod_bsup no_control_l_def
+            split: md_prio.splits prod.splits md_triv.splits option.splits list.split_asm)
+
+        have Conc' : "safe_for gs m' npost"
+          using guardediD[OF Guard, of "m'"] Hpay' Cont_final'
+          unfolding Pay_final Cont_final' lift_pred_valid_s_def lift_pred_s_def lift_pred_validx_s_def
+          using lifting_validDO[OF Valid'] lifting_validDP[OF Valid'] lifting_validxDP'[OF Valid Hpay3]
+          by(cases m; auto)
+
+        have Inl_alt : "sem_step_p gs m m'"
+          using Inl unfolding sem_step_p_eq by simp
+
+        show  "safe_for gs m npost"
+          using safe_for_weaken[OF safe_for_extend[OF Conc' Excp_1[OF Inl_alt]], of npost]
+          by simp
+      qed
+    qed
+  qed
+
+  thus "\<exists>npre.
+          |#gs#| {#-lift_pred_validx_s id l S c
+                     P1, (npre + npost)-#} [G c z] {#-lift_pred_validx_s id l S c P2, npost-#}"
+    by blast
+qed
+
+(*
+lemma HTS_imp_HT'' :
   assumes H: "f % {{P1}} c {{P2}}"
   assumes Valid : "lifting_valid l S"
   assumes Hf' : "f' = no_control_l l f"
@@ -68,26 +289,26 @@ lemma HTS_imp_HT' :
   assumes Skip : "lfts c = Sskip"
   assumes Hnemp : "g \<in> (set fs - {seq_sem_l_gen lfts})"
   assumes Hdom : "(f' \<downharpoonleft> (set fs - {seq_sem_l_gen lfts}) c)"
-  shows "|gs| {~ (lift_pred_valid_s id l S c P1) ~} [G c z] {~ (lift_pred_valid_s id l S c P2) ~}"
+  shows "|gs| {~ (lift_pred_s id l c P1) ~} [G c z] {~ (lift_pred_s id l c P2) ~}"
 proof(rule HT'I)
   fix npost
 
-  have "|#gs#| {#-lift_pred_valid_s id l S c
+  have "|#gs#| {#-lift_pred_s id l c
                      P1, (0 +
-                          npost)-#} [G c z] {#-lift_pred_valid_s id l S c
+                          npost)-#} [G c z] {#-lift_pred_s id l c
        P2, npost-#}"
     unfolding add_0
   proof
     fix c'
 
-    assume Guard : "|#gs#| {#lift_pred_valid_s id l S c P2, npost#} c'"
-    show "|#gs#| {#lift_pred_valid_s id l S c P1, npost#} ([G c z] @ c')"
+    assume Guard : "|#gs#| {#lift_pred_s id l c P2, npost#} c'"
+    show "|#gs#| {#lift_pred_s id l c P1, npost#} ([G c z] @ c')"
     proof
       fix m :: "('a, 'c) control"
-      assume Hpay : "lift_pred_valid_s id l S c P1 (payload m)"
+      assume Hpay : "lift_pred_s id l c P1 (payload m)"
       assume Hcont : "cont m = Inl ([G c z] @ c') "
 
-      have Hpay1 : "P1 (LOut l c (payload m))" and Hpay2 : "payload m \<in> S c"
+      have Hpay1 : "P1 (LOut l c (payload m))" 
         using Hpay
         unfolding lift_pred_valid_s_def lift_pred_s_def
         by auto
@@ -197,7 +418,8 @@ proof(rule HT'I)
           "rest <[ LUpd l c (f c (LOut l c rest)) rest"
           using lifting_validDI[OF Valid Rest]
           by auto
-
+(* TODO: I think the problem here is that we actually need to use the fact that we want a more
+restricted set than just what we are valid on... *)
         have LUpd_rest2 : "[^ LUpd l c (f c (LOut l c rest)) rest, rest ^] = LUpd l c (f c (LOut l c rest)) rest"
           using bsup_base_leq2[OF LUpd_rest1]
           by simp
@@ -262,4 +484,6 @@ proof(rule HT'I)
                      P1, (npre + npost)-#} [G c z] {#-lift_pred_valid_s id l S c P2, npost-#}"
     by blast
 qed
+*)
+
 end
