Lifter/LifterX.thy
@@ -1,0 +1,260 @@
+theory LifterX
+imports Lifter Lifter_Instances
+begin
+
+(* An experiment in developing a variant of Lifter that
+has a weaker notion of valid-sets (updates don't unconditionally need to be in the valid set;
+instead this is only the case if we started with a valid input
+*)
+
+class Okay =
+  fixes ok_S :: "'a set"
+
+instantiation md_triv :: (_) Okay
+begin
+definition triv_ok_S : "(ok_S :: 'a md_triv set) = UNIV"
+instance proof qed
+end
+
+instantiation md_prio :: (Okay) Okay
+begin
+definition prio_ok_S : "(ok_S :: 'a md_prio set) = { x :: 'a md_prio . \<exists> x' p' . x = mdp p' x' \<and> x' \<in> ok_S }"
+instance proof qed
+end
+
+instantiation option :: (Okay) Okay
+begin
+definition option_ok_S : "(ok_S :: 'a option set) = (Some ` ok_S)"
+instance proof qed
+end
+
+instantiation prod :: (Okay, Okay) Okay
+begin
+definition prod_ok_S : "(ok_S :: ('a * 'b) set) = { x :: 'a * 'b . \<exists> a' b' . x = (a', b') \<and> a' \<in> ok_S \<and> b' \<in> ok_S}"
+instance proof qed
+end
+
+(* idea:
+   - normal validity
+   - valid_set has certain relation (superset) to Okay set
+   - (thus, law 2 still works even if we assume Okay-ness)
+   - tighter law 3: if b is in Okay, then so is LUpd l s a b.
+*)
+definition lifting_validx_weak ::
+  "('x, 'a, 'b :: {Pord, Okay}, 'z) lifting_scheme \<Rightarrow> ('x, 'b) valid_set \<Rightarrow> bool" where
+"lifting_validx_weak l S =
+ ((lifting_valid_weak l S) \<and>
+  (\<forall> s . ok_S \<subseteq> S s) \<and>
+  (\<forall> s a b . b \<in> ok_S \<longrightarrow> LUpd l s a b \<in> ok_S))"
+
+lemma lifting_validx_weakI :
+  assumes HV : "lifting_valid_weak l S"
+  assumes HS : "\<And> s . ok_S \<subseteq> S s"
+  assumes HP' : "\<And> s a b . b \<in> ok_S \<Longrightarrow> LUpd l s a b \<in> ok_S"
+  shows "lifting_validx_weak l S"
+  using assms
+  by(auto simp add: lifting_validx_weak_def)
+
+lemma lifting_validx_weakDV :
+  assumes H : "lifting_validx_weak l S"
+  shows "lifting_valid_weak l S"
+  using assms
+  by(auto simp add: lifting_validx_weak_def)
+
+lemma lifting_validx_weakDS :
+  assumes H : "lifting_validx_weak l S"
+  shows "ok_S \<subseteq> S s"
+  using assms
+  by(auto simp add: lifting_validx_weak_def)
+
+lemma lifting_validx_weakDP' :
+  assumes H : "lifting_validx_weak l (S :: ('a \<Rightarrow> ('b :: {Pord, Okay}) set))"
+  assumes Hok : "(b :: 'b) \<in> ok_S"
+  shows "LUpd l s a b \<in> ok_S"
+  using assms
+  by(auto simp add: lifting_validx_weak_def)
+
+definition lifting_validx_weakb ::
+  "('x, 'a, 'b :: {Pordb, Okay}, 'z) lifting_scheme \<Rightarrow> ('x, 'b) valid_set \<Rightarrow> bool" where
+"lifting_validx_weakb l S =
+ ((lifting_valid_weakb l S) \<and>
+  (\<forall> s . ok_S \<subseteq> S s) \<and>
+  (\<forall> s a b . b \<in> ok_S \<longrightarrow> LUpd l s a b \<in> ok_S))"
+
+lemma lifting_validx_weakbI :
+  assumes HV : "lifting_valid_weakb l S"
+  assumes HS : "\<And> s . ok_S \<subseteq> S s"
+  assumes HP' : "\<And> s a b . b \<in> ok_S \<Longrightarrow> LUpd l s a b \<in> ok_S"
+  shows "lifting_validx_weakb l S"
+  using assms
+  by(auto simp add: lifting_validx_weakb_def)
+
+lemma lifting_validx_weakbDV :
+  assumes H : "lifting_validx_weakb l S"
+  shows "lifting_valid_weakb l S"
+  using assms
+  by(auto simp add: lifting_validx_weakb_def)
+
+lemma lifting_validx_weakbDS :
+  assumes H : "lifting_validx_weakb l S"
+  shows "ok_S \<subseteq> S s"
+  using assms
+  by(auto simp add: lifting_validx_weakb_def)
+
+lemma lifting_validx_weakbDP' :
+  assumes H : "lifting_validx_weakb l (S :: ('a \<Rightarrow> ('b :: {Pordb, Okay}) set))"
+  assumes Hok : "(b :: 'b) \<in> ok_S"
+  shows "LUpd l s a b \<in> ok_S"
+  using assms
+  by(auto simp add: lifting_validx_weakb_def)
+
+definition lifting_validx ::
+  "('x, 'a, 'b :: {Pord, Okay}, 'z) lifting_scheme \<Rightarrow> ('x, 'b) valid_set \<Rightarrow> bool" where
+"lifting_validx l S =
+ ((lifting_valid l S) \<and>
+  (\<forall> s . ok_S \<subseteq> S s) \<and>
+  (\<forall> s a b . b \<in> ok_S \<longrightarrow> LUpd l s a b \<in> ok_S))"
+
+lemma lifting_validxI :
+  assumes HV : "lifting_valid l S"
+  assumes HS : "\<And> s . ok_S \<subseteq> S s"
+  assumes HP' : "\<And> s a b . b \<in> ok_S \<Longrightarrow> LUpd l s a b \<in> ok_S"
+  shows "lifting_validx l S"
+  using assms
+  by(auto simp add: lifting_validx_def)
+
+lemma lifting_validxDV :
+  assumes H : "lifting_validx l S"
+  shows "lifting_valid l S"
+  using assms
+  by(auto simp add: lifting_validx_def)
+
+lemma lifting_validxDS :
+  assumes H : "lifting_validx l S"
+  shows "ok_S \<subseteq> S s"
+  using assms
+  by(auto simp add: lifting_validx_def)
+
+lemma lifting_validxDP' :
+  assumes H : "lifting_validx l (S :: ('a \<Rightarrow> ('b :: {Pord, Okay}) set))"
+  assumes Hok : "(b :: 'b) \<in> ok_S"
+  shows "LUpd l s a b \<in> ok_S"
+  using assms
+  by(auto simp add: lifting_validx_def)
+
+definition lifting_validxb ::
+  "('x, 'a, 'b :: {Pordb, Okay}, 'z) lifting_scheme \<Rightarrow> ('x, 'b) valid_set \<Rightarrow> bool" where
+"lifting_validxb l S =
+ ((lifting_validb l S) \<and>
+  (\<forall> s . ok_S \<subseteq> S s) \<and>
+  (\<forall> s a b . b \<in> ok_S \<longrightarrow> LUpd l s a b \<in> ok_S))"
+
+lemma lifting_validxbI :
+  assumes HV : "lifting_validb l S"
+  assumes HS : "\<And> s . ok_S \<subseteq> S s"
+  assumes HP' : "\<And> s a b . b \<in> ok_S \<Longrightarrow> LUpd l s a b \<in> ok_S"
+  shows "lifting_validxb l S"
+  using assms
+  by(auto simp add: lifting_validxb_def)
+
+lemma lifting_validxbDV :
+  assumes H : "lifting_validxb l S"
+  shows "lifting_validb l S"
+  using assms
+  by(auto simp add: lifting_validxb_def)
+
+lemma lifting_validxbDS :
+  assumes H : "lifting_validxb l S"
+  shows "ok_S \<subseteq> S s"
+  using assms
+  by(auto simp add: lifting_validxb_def)
+
+lemma lifting_validxbDP' :
+  assumes H : "lifting_validxb l (S :: ('a \<Rightarrow> ('b :: {Pordb, Okay}) set))"
+  assumes Hok : "(b :: 'b) \<in> ok_S"
+  shows "LUpd l s a b \<in> ok_S"
+  using assms
+  by(auto simp add: lifting_validxb_def)
+
+(* Problem: how does this affect the first law (LOut (LUpd ...))
+we might be able to keep this the same. However, I can't get over the fact that this
+feels wrong...
+*)
+
+lemma triv_l_validx_weak :
+  shows "lifting_validx_weak (triv_l :: ('x, 'a :: Bogus, 'a md_triv) lifting) (\<lambda> _ . UNIV)"
+proof(rule lifting_validx_weakI)
+  show "lifting_valid_weak' triv_l" using triv_l_valid_weak by auto
+next
+  fix s
+  show "ok_S \<subseteq> UNIV" using triv_ok_S
+    by(auto)
+next
+  show "\<And>s a b. b \<in> ok_S \<Longrightarrow> LUpd triv_l s a b \<in> ok_S"
+    by(auto simp add: triv_ok_S)
+qed
+
+lemma option_l_validx_weak :
+  assumes H : "lifting_validx_weak (t :: ('x, 'a, 'b :: {Pord, Okay}, 'z) lifting_scheme) S"
+  shows "lifting_validx_weak (option_l t) (option_l_S S)"
+proof(rule lifting_validx_weakI)
+  show "lifting_valid_weak (option_l t)
+     (option_l_S S)"
+    using option_l_valid_weak lifting_validx_weakDV[OF H] by auto
+next
+  show "\<And> s . ok_S \<subseteq> option_l_S S s"
+    using lifting_validx_weakDS[OF H]
+    by(auto simp add: option_l_S_def option_ok_S)
+next
+  show "\<And>s a b.
+       b \<in> ok_S \<Longrightarrow>
+       LUpd (option_l t) s a b \<in> ok_S"
+    using lifting_validx_weakDP'[OF H]
+    by(auto simp add: option_l_def option_l_S_def option_ok_S)
+qed
+
+(* TODO: option_l_valid, option_l_validb *)
+
+lemma fst_l_validx_weak :
+  assumes H : "lifting_validx_weak (t :: ('x, 'a, 'b :: {Pord, Okay}, 'z) lifting_scheme) S"
+  shows "lifting_validx_weak (fst_l t) (fst_l_S S)"
+proof(rule lifting_validx_weakI)
+  show "lifting_valid_weak (fst_l t) (fst_l_S S)"
+    using lifting_validx_weakDV[OF H] fst_l_valid_weak by auto
+next
+  show "\<And>s. ok_S \<subseteq> fst_l_S S s"
+    using lifting_validx_weakDS[OF H]
+    by(auto simp add: fst_l_S_def prod_ok_S)
+next
+  show "\<And>s a b.
+         b \<in> ok_S \<Longrightarrow> LUpd (fst_l t) s a b \<in> ok_S"
+    using lifting_validx_weakDP'[OF H]
+    by(auto simp add: fst_l_def fst_l_S_def prod_ok_S)
+qed
+
+(* TODO: other variants of fst; snd as well *)
+
+lemma merge_l_validx_gen :
+  assumes H1 : "lifting_validx (l1 :: ('x, 'a1, 'b :: {Mergeable, Okay}, 'z1) lifting_scheme) S1"
+  assumes H2 : "lifting_validx (l2 :: ('x, 'a2, 'b :: {Mergeable, Okay}, 'z2) lifting_scheme) S2"
+  assumes Hort : "l_ortho_alt l1 S1 l2 S2"
+  shows "lifting_validx (merge_l l1 l2) (\<lambda> s . S1 s \<inter> S2 s)"
+proof(rule lifting_validxI)
+  show "lifting_valid (merge_l l1 l2) (\<lambda>s. S1 s \<inter> S2 s)"
+    using merge_l_valid_gen[OF lifting_validxDV[OF H1] lifting_validxDV[OF H2] Hort]
+    by auto
+next
+  show "\<And> s . ok_S \<subseteq> S1 s \<inter> S2 s"
+    using lifting_validxDS[OF H1] lifting_validxDS[OF H2]
+      prod_ok_S
+    by(auto)
+next
+  show "\<And>s a b.
+       b \<in> ok_S \<Longrightarrow>
+       LUpd (merge_l l1 l2) s a b \<in> ok_S"
+    using lifting_validxDP'[OF H1] lifting_validxDP'[OF H2]
+    by(auto simp add: merge_l_def)
+qed
+
+
+end
